fix cellio

cellio/MainIAproof.v
@@ -5,54 +5,42 @@ Set Implicit Arguments.
 
 Module MainIA. Section MainIA.
   Import CellioA.
-  Context `{!crisG Γ Σ α β τ _S _I}.
-  Context `{_cellioG: !cellioG}.
+  Context `{!crisG Γ Σ α β τ _S _I, !concGS, !cellioG}.
 
-  Definition Ist: alist key Any.t -> alist key Any.t -> iProp Σ :=
-    λ st_src st_tgt, emp%I.
+  Context (sp: specmap).
+  Context (sp_input: sp !! speckey_fn CtxHdr.input = None).
+  Context (sp_foo: sp !! speckey_fn CtxHdr.foo = None).
 
-  Context (sp: sp_type).
-  Context (sp_input: sp CtxHdr.input = None).
-  Context (sp_foo: sp CtxHdr.foo = None).
-  
   Local Definition CellioA := (CellioA.t).
   Local Definition MainA := (MainA.t sp).
-  Local Definition IstFull := (IstProd (IstSB MainA.(Mod.scopes) Ist) IstEq).
+  Local Definition IstFull := (IstProd (IstSB MainA.(Mod.scopes) IstTrue) IstEq).
 
   Lemma simF_main:
-    ISim.sim_fun open MainA (MainI.t ★ CellioA) MainA.init_cond IstFull None.
+    ISim.sim_fun open MainA (MainI.t ★ CellioA) IstFull None.
   Proof using sp_input sp_foo.
-    init_simF.
-    
-    (* Take cell(0) *)
-    steps_l. 
-    iDestruct "IST" as "[IST ASM]"; subst.
+    iStartSim. unfold MainI.main, MainA.main.
 
-    steps_r. inline_r.
+    (* Take cell(0) *)
+    steps_l. iDestruct "ASM" as "[-> CELL]".
+
+    steps_r. inline_r. unfold CellioA.set.
     (* Give cell(0) *)
-    steps_r. forces_r. iSplitL ""; eauto.
-    forces_r. iSplitL "ASM"; eauto.
+    steps_r. forces_r. iSplit; et.
+    forces_r. iSplitL "CELL"; et.
 
     (* Call Input() simultaneously *)
     steps_r. rewrite sp_input.
-    call "IST". 
-    {
-      iDestruct "IST" as "[-> ->]".
-      repeat iExists []. iSplit; eauto;
-      repeat unfold_mod; ss;
-      repeat (iSplit; eauto); iPureIntro; prove_scope.
-    }
-    steps_l. steps_r. hss.
+    call "IST". iIntros (r0 st_src0 st_tgt0) "IST".
+    steps_l. steps_r. destruct Any.downcast; [|steps_l; ss]. hss.
 
     (* Take cell(i) *)
     steps_r. iDestruct "GRT'" as "%". subst. hss.
     
     (* Call Foo.foo() simultaneously *)
-    steps_r. rewrite sp_foo.
-    call "IST"; eauto.
-    steps_l. hss. steps_r. hss. steps_r.
-
-    inline_r.
+    steps_r. steps_l. rewrite sp_foo.
+    call "IST". iIntros (r1 st_src1 st_tgt1) "IST".
+    steps_l. steps_r. destruct Any.downcast; [|steps_l; ss]. hss.
+    steps_r. inline_r. unfold CellioA.get.
     (* Give cell(i) *)
     step_r. forces_r. iSplitL ""; eauto.
     forces_r. iSplitL "GRT"; eauto.
@@ -63,16 +51,18 @@ Module MainIA. Section MainIA.
     (* Call Print(i) simultaneously *)
     steps_r. step.
 
-    steps_l. steps_r. step. eauto.
+    forces_l. iSplit; et.
+    step. iFrame. ss.
 
     Unshelve. all:(exact ()).
   (*SLOW*)Qed.
 
   Theorem sim :
-    ISim.t open MainA (MainI.t ★ CellioA) MainA.init_cond IstFull.
+    ISim.t open MainA (MainI.t ★ CellioA) emp%I IstFull.
   Proof using sp_input sp_foo.
     init_sim.
-    (* - exfalso. revert H. rewrite /MainI.t /CellioA. unseal CRIS; ss. *)
+    - iIntros "_". unfold IstFull, IstProd.
+      iExists ∅, ∅, ∅, ∅. ss.
     - eapply simF_main; eauto.
   Qed.
 End MainIA. End MainIA.
